src/model/Reserves.v
@@ -14,23 +14,76 @@ Require Import Time.
 Set Implicit Arguments.
 
 
+(* TODO: move to promising-lib *)
+
+Variant option_le (A: Type) (le: A -> A -> Prop): forall (lhs rhs: option A), Prop :=
+| option_le_None
+    rhs:
+  option_le le None rhs
+| option_le_Some
+    lhs rhs
+    (LE: le lhs rhs):
+  option_le le (Some lhs) (Some rhs)
+.
+#[export] Hint Constructors option_le: core.
+
+#[export] Program Instance option_le_PreOrder A (le: A -> A -> Prop) `{PreOrder A le}:
+  PreOrder (option_le le).
+Next Obligation.
+  ii. destruct x; eauto. econs. refl.
+Qed.
+Next Obligation.
+  ii. inv H0; inv H1; eauto. econs. etrans; eauto.
+Qed.
+
+Definition option_join (A: Type) (join: A -> A -> A) (lhs rhs: option A): option A :=
+  match lhs, rhs with
+  | None, _ => rhs
+  | _, None => lhs
+  | Some l, Some r => Some (join l r)
+  end.
+
+Lemma option_join_comm
+      A (join: A -> A -> A)
+      (COMM: forall x y, join x y = join y x):
+  forall x y, option_join join x y = option_join join y x.
+Proof.
+  i. destruct x, y; ss. f_equal. auto.
+Qed.
+
+Lemma option_join_assoc
+      A (join: A -> A -> A)
+      (ASSOC: forall x y z, join (join x y) z = join x (join y z)):
+  forall x y z,
+    option_join join (option_join join x y) z =
+    option_join join x (option_join join y z).
+Proof.
+  i. destruct x, y, z; ss. f_equal. auto.
+Qed.
+
+Lemma option_join_spec
+      A (le: A -> A -> Prop) (join: A -> A -> A)
+      (SPEC: forall x y o, le x o -> le y o -> le (join x y) o):
+  forall x y o,
+    option_le le x o -> option_le le y o ->
+    option_le le (option_join join x y) o.
+Proof.
+  i. inv H; inv H0; econs; eauto.
+Qed.
+
+
 Module Reserves.
   Definition t := Loc.t -> option Time.t.
 
   Definition eq := @eq t.
 
-  Definition le (lhs rhs: t): Prop :=
+  Definition incl (lhs rhs: t): Prop :=
     forall loc ts (LHS: lhs loc = Some ts),
       rhs loc = Some ts.
 
-  Global Program Instance le_PreOrder: PreOrder le.
-  Next Obligation. ii. ss. Qed.
-  Next Obligation. ii. eauto. Qed.
-  #[global] Hint Resolve le_PreOrder_obligation_2: core.
-
-  Lemma antisym l r
-        (LR: le l r)
-        (RL: le r l):
+  Lemma incl_antisym l r
+        (LR: incl l r)
+        (RL: incl r l):
     l = r.
   Proof.
     extensionality loc.
@@ -39,11 +92,24 @@ Module Reserves.
     exploit LR; eauto.
   Qed.
 
-  Definition bot: t := fun _ => None.
+  Global Program Instance incl_PreOrder: PreOrder incl.
+  Next Obligation. ii. ss. Qed.
+  Next Obligation. ii. eauto. Qed.
+  #[global] Hint Resolve incl_PreOrder_obligation_2: core.
 
-  Lemma bot_spec (tm:t): le bot tm.
+  Definition le (lhs rhs: t): Prop :=
+    forall loc, option_le Time.le (lhs loc) (rhs loc).
+
+  Lemma le_antisym l r
+        (LR: le l r)
+        (RL: le r l):
+    l = r.
   Proof.
-    ii. ss.
+    extensionality loc.
+    specialize (LR loc). specialize (RL loc).
+    inv LR; inv RL; try congr.
+    rewrite <- H0, <- H in *. clarify.
+    f_equal. apply TimeFacts.antisym; ss.
   Qed.
 
   Definition disjoint (x y: t): Prop :=
@@ -57,15 +123,27 @@ Module Reserves.
     ii. eauto.
   Qed.
 
-  Lemma bot_disjoint prom: disjoint bot prom.
-  Proof.
-    ii. ss.
-  Qed.
-
   Definition finite (rsv: t): Prop :=
     exists dom,
     forall loc ts (GET: rsv loc = Some ts),
       List.In loc dom.
+
+  Definition bot: t := fun _ => None.
+
+  Lemma bot_incl (rsv: t): incl bot rsv.
+  Proof.
+    ii. ss.
+  Qed.
+
+  Lemma bot_le (rsv: t): le bot rsv.
+  Proof.
+    ii. econs.
+  Qed.
+
+  Lemma bot_disjoint prom: disjoint bot prom.
+  Proof.
+    ii. ss.
+  Qed.
 
   Lemma bot_finite: finite bot.
   Proof.
@@ -87,14 +165,14 @@ Module Reserves.
 
   Variant reserve (rsv1 grsv1: t) (loc: Loc.t) (ts: Time.t) (rsv2 grsv2: t): Prop :=
   | reserve_intro
-      (RSV: add rsv1 loc ts rsv2)
-      (GRSV: add grsv1 loc ts grsv2)
+      (ADD: add rsv1 loc ts rsv2)
+      (GADD: add grsv1 loc ts grsv2)
   .
 
   Variant cancel (rsv1 grsv1: t) (loc: Loc.t) (ts: Time.t) (rsv2 grsv2: t): Prop :=
   | cancel_intro
-      (RSV: remove rsv1 loc ts rsv2)
-      (GRSV: remove grsv1 loc ts grsv2)
+      (REMOVE: remove rsv1 loc ts rsv2)
+      (GREMOVE: remove grsv1 loc ts grsv2)
   .
 
 
@@ -175,25 +253,25 @@ Module Reserves.
     condtac; ss; eauto.
   Qed.
 
-  Lemma reserve_le
+  Lemma reserve_incl
         rsv1 grsv1 loc ts rsv2 grsv2
         (RESERVE: reserve rsv1 grsv1 loc ts rsv2 grsv2)
-        (LE1: le rsv1 grsv1):
-    le rsv2 grsv2.
+        (LE1: incl rsv1 grsv1):
+    incl rsv2 grsv2.
   Proof.
     ii. revert LHS.
-    inv RESERVE. inv RSV. inv GRSV.
+    inv RESERVE. inv ADD. inv GADD.
     unfold LocFun.add. condtac; ss. eauto.
   Qed.
 
-  Lemma cancel_le
+  Lemma cancel_incl
         rsv1 grsv1 loc ts rsv2 grsv2
         (CANCEL: cancel rsv1 grsv1 loc ts rsv2 grsv2)
-        (LE1: le rsv1 grsv1):
-    le rsv2 grsv2.
+        (LE1: incl rsv1 grsv1):
+    incl rsv2 grsv2.
   Proof.
     ii. revert LHS.
-    inv CANCEL. inv RSV. inv GRSV.
+    inv CANCEL. inv REMOVE. inv GREMOVE.
     unfold LocFun.add. condtac; ss. eauto.
   Qed.
 
@@ -201,12 +279,12 @@ Module Reserves.
         rsv1 grsv1 loc ts rsv2 grsv2
         ctx
         (RESERVE: reserve rsv1 grsv1 loc ts rsv2 grsv2)
-        (LE_CTX: le ctx grsv1)
+        (LE_CTX: incl ctx grsv1)
         (DISJOINT: disjoint rsv1 ctx):
     (<<DISJOINT: disjoint rsv2 ctx>>) /\
-    (<<LE_CTX: le ctx grsv2>>).
+    (<<LE_CTX: incl ctx grsv2>>).
   Proof.
-    inv RESERVE. inv RSV. inv GRSV. splits; ii.
+    inv RESERVE. inv ADD. inv GADD. splits; ii.
     - revert GET1. unfold LocFun.add.
       condtac; ss; subst; eauto. i. clarify.
       exploit LE_CTX; eauto. i. congr.
@@ -218,12 +296,12 @@ Module Reserves.
         rsv1 grsv1 loc ts rsv2 grsv2
         ctx
         (CANCEL: cancel rsv1 grsv1 loc ts rsv2 grsv2)
-        (LE_CTX: le ctx grsv1)
+        (LE_CTX: incl ctx grsv1)
         (DISJOINT: disjoint rsv1 ctx):
     (<<DISJOINT: disjoint rsv2 ctx>>) /\
-    (<<LE_CTX: le ctx grsv2>>).
+    (<<LE_CTX: incl ctx grsv2>>).
   Proof.
-    inv CANCEL. inv RSV. inv GRSV. splits; ii.
+    inv CANCEL. inv REMOVE. inv GREMOVE. splits; ii.
     - revert GET1. unfold LocFun.add.
       condtac; ss; subst; eauto.
     - unfold LocFun.add. condtac; ss; subst; eauto.
